books/kestrel/arm/encodings.lisp
@@ -82,19 +82,22 @@
     (:bic-register (cond 4) 0 0 _ 0 _ 1 1 1 0 s (rn 4) (rd 4) (imm5 5) (type 2) 0 (rm 4))
     (:bic-register-shifted-register (cond 4) 0 0 _ 0 _ 1 1 1 0 s (rn 4) (rd 4) (rs 4) 0 (type 2) 1 (rm 4))
 
-    ;; todo: bkpt
+    ;; todo: bkpt ; software breakpoint
 
-    (:bl  (cond 4) 1 0 1 1 (imm24 24)) ;; Encoding A1 of BL/BLX (immediate)
+    (:bl (cond 4) 1 0 1 1 (imm24 24)) ;; Encoding A1 of BL/BLX (immediate)
+    (:blx-immediate  1 1 1 1 _ 1 0 1 h (imm24 24)) ;; Encoding A2 of BL/BLX (immediate)
+    (:blx-register (cond 4) 0 0 0 1 0 0 1 0 (1) (1) (1) (1) _ (1) (1) (1) (1)_ (1) (1) (1) (1) 0 0 1 1 (rm 4))
 
-;;;    (:blx-immediate  1 1 1 1 1 0 1 h (imm24 24)) ;; Encoding A2 of BL/BLX (immediate)
 ;;;    (:blx-register  (cond 4) 0 0 0 1 0 0 1 0 _ (1) (1) (1) (1) _ (1) (1) (1) (1) _ (1) (1) (1) (1) _ 0 0 1 1 (rm 4))
 
     (:bx (cond 4) 0 0 0 1 0 0 1 0 _ (1) (1) (1) (1) _ (1) (1) (1) (1) _ (1) (1) (1) (1) _ 0 0 0 1 (rm 4))
 
-    ;; todo: bxj
-    ;; todo: cdp/cdp2
-    ;; todo: clrex
-    ;; todo: clz
+    ;; todo: bxj ; involves Jazelle
+    ;; todo: cbnz, cbz
+    ;; todo: cdp/cdp2 ; involves Coprocessor
+    ;; todo: clrex ; involves exclusive monitors
+
+    (:clz (cond 4) 0 0 0 1 0 1 1 0 (1) (1) (1) (1) (rd 4) (1) (1) (1) (1) 0 0 0 1 (rm 4))
 
     (:cmn-immediate (cond 4) 0 0 _ 1 _ 1 0 1 1 _ 1 (rn 4) (0) (0) (0) (0) (imm12 12))
     (:cmn-register  (cond 4) 0 0 _ 0 _ 1 0 1 1 _ 1 (rn 4) (0) (0) (0) (0) (imm5 5) (type 2) 0 (rm 4))
@@ -104,72 +107,72 @@
     (:cmp-register  (cond 4) 0 0 _ 0 _ 1 0 1 0 _ 1 (rn 4) (0) (0) (0) (0) (imm5 5) (type 2) 0 (rm 4))
     (:cmp-register-shifted-register (cond 4) 0 0 _ 0 _ 1 0 1 0 _ 1 (rn 4) (0) (0) (0) (0) (rs 4) 0 (type 2) 1 (rm 4))
 
-    ;; todo: csdb
-    ;; todo: dbg
-    ;; todo: dmb
-    ;; todo: dsb
+    ;; todo: csdb ; memory barrier
+    ;; todo: dbg ; debug hint
+    ;; todo: dmb ; memory barrier
+    ;; todo: dsb ; memory barrier
 
     (:eor-immediate  (cond 4) 0 0 1 0 0 0 1 s (rn 4) (rd 4) (imm12 12))
     (:eor-register   (cond 4) 0 0 0 0 0 0 1 s (rn 4) (rd 4) (imm5 5) (type 2) 0 (rm 4))
     (:eor-register-shifted-register   (cond 4) 0 0 0 0 0 0 1 s (rn 4) (rd 4) (rs 4) 0 (type 2) 1 (rm 4))
 
-    ;; todo: isb
-    ;; todo: ldc/ldc2
+    ;; todo: isb ; pipeline flush
+    ;; todo: ldc/ldc2 ; coprocessor
 
     (:ldm/ldmia/ldmfd (cond 4) 1 0 0 0 1 0 w 1 (rn 4) (register_list 16))
-;;;    (:ldmda/ldmfa     (cond 4) 1 0 0 0 0 0 w 1 (rn 4) (register_list 16))
-;;;    (:ldmdb/ldmea     (cond 4) 1 0 0 1 0 0 w 1 (rn 4) (register_list 16))
+    (:ldmda/ldmfa     (cond 4) 1 0 0 0 0 0 w 1 (rn 4) (register_list 16))
+    (:ldmdb/ldmea     (cond 4) 1 0 0 1 0 0 w 1 (rn 4) (register_list 16))
     (:ldmib/ldmed     (cond 4) 1 0 0 1 1 0 w 1 (rn 4) (register_list 16))
 
     (:ldr-immediate  (cond 4) 0 1 0 p u 0 w 1 (rn 4) (rt 4) (imm12 12))
     (:ldr-literal    (cond 4) 0 1 0 p u 0 w 1 1 1 1 1 (rt 4) (imm12 12))
-    (:ldr-register    (cond 4) 0 1 1 p u 0 w 1 (rn 4) (rt 4) (imm5 5) (type 2) 0 (rm 4))
+    (:ldr-register   (cond 4) 0 1 1 p u 0 w 1 (rn 4) (rt 4) (imm5 5) (type 2) 0 (rm 4))
 
     (:ldrb-immediate  (cond 4) 0 1 0 p u 1 w 1 (rn 4) (rt 4) (imm12 12))
-    (:ldrb-literal  (cond 4) 0 1 0 p u 1 w 1 1 1 1 1 (rt 4) (imm12 12))
-    (:ldrb-register  (cond 4) 0 1 1 p u 1 w 1 (rn 4) (rt 4) (imm5 5) (type 2) 0 (rm 4))
+    (:ldrb-literal    (cond 4) 0 1 0 p u 1 w 1 1 1 1 1 (rt 4) (imm12 12))
+    (:ldrb-register   (cond 4) 0 1 1 p u 1 w 1 (rn 4) (rt 4) (imm5 5) (type 2) 0 (rm 4))
 
-    (:ldrbt-encoding-a1  (cond 4) 0 1 0 0 u 1 1 1 (rn 4) (rt 4) (imm12 12))
-    (:ldrbt-encoding-a2  (cond 4) 0 1 1 0 u 1 1 1 (rn 4) (rt 4) (imm5 5) (type 2) 0 (rm 4))
+    (:ldrbt-encoding-a1 (cond 4) 0 1 0 0 u 1 1 1 (rn 4) (rt 4) (imm12 12))
+    (:ldrbt-encoding-a2 (cond 4) 0 1 1 0 u 1 1 1 (rn 4) (rt 4) (imm5 5) (type 2) 0 (rm 4))
 
-    (:ldrd-immediate  (cond 4) 0 0 0 p u 1 w 0 (rn 4) (rt 4) (imm4h 4) 1 1 0 1 (imm4l 4))
-    (:ldrd-literal    (cond 4) 0 0 0 (1) u 1 (0) 0 1 1 1 1 (rt 4) (imm4h 4) 1 1 0 1 (imm4l 4))
-    (:ldrd-register   (cond 4) 0 0 0 p u 0 w 0 (rn 4) (rt 4) (0) (0) (0) (0) 1 1 0 1 (rm 4))
+    (:ldrd-immediate (cond 4) 0 0 0 p u 1 w 0 (rn 4) (rt 4) (imm4h 4) 1 1 0 1 (imm4l 4))
+    (:ldrd-literal   (cond 4) 0 0 0 (1) u 1 (0) 0 1 1 1 1 (rt 4) (imm4h 4) 1 1 0 1 (imm4l 4))
+    (:ldrd-register  (cond 4) 0 0 0 p u 0 w 0 (rn 4) (rt 4) (0) (0) (0) (0) 1 1 0 1 (rm 4))
 
 ;;;    (:ldrex    (cond 4) 0 0 0 1 1 0 0 1 (rn 4) (rt 4) (1) (1) (1) (1) 1 0 0 1 (1) (1) (1) (1))
 ;;;    (:ldrexb   (cond 4) 0 0 0 1 1 1 0 1 (rn 4) (rt 4) (1) (1) (1) (1) 1 0 0 1 (1) (1) (1) (1))
 ;;;    (:ldrexd   (cond 4) 0 0 0 1 1 0 1 1 (rn 4) (rt 4) (1) (1) (1) (1) 1 0 0 1 (1) (1) (1) (1))
 ;;;    (:ldrexh   (cond 4) 0 0 0 1 1 1 1 1 (rn 4) (rt 4) (1) (1) (1) (1) 1 0 0 1 (1) (1) (1) (1))
 
-    (:ldrh-immediate  (cond 4) 0 0 0 p u 1 w 1 (rn 4) (rt 4) (imm4h 4) 1 0 1 1 (imm4l 4))
-    (:ldrh-literal    (cond 4) 0 0 0 p u 1 w 1 1 1 1 1 (rt 4) (imm4h 4) 1 0 1 1 (imm4l 4))
-    (:ldrh-register   (cond 4) 0 0 0 p u 0 w 1 (rn 4) (rt 4) (0) (0) (0) (0) 1 0 1 1 (rm 4))
+    (:ldrh-immediate (cond 4) 0 0 0 p u 1 w 1 (rn 4) (rt 4) (imm4h 4) 1 0 1 1 (imm4l 4))
+    (:ldrh-literal   (cond 4) 0 0 0 p u 1 w 1 1 1 1 1 (rt 4) (imm4h 4) 1 0 1 1 (imm4l 4))
+    (:ldrh-register  (cond 4) 0 0 0 p u 0 w 1 (rn 4) (rt 4) (0) (0) (0) (0) 1 0 1 1 (rm 4))
 
-    (:ldrht-encoding-a1  (cond 4) 0 0 0   0 u 1   1   1 (rn 4) (rt 4) (imm4h 4) 1 0 1 1 (imm4l 4))
-    (:ldrht-encoding-a2  (cond 4) 0 0 0 _ 0 u 0 _ 1 _ 1 (rn 4) (rt 4) (0) (0) (0) (0) 1 0 1 1 (rm 4))
+    (:ldrht-encoding-a1 (cond 4) 0 0 0   0 u 1   1   1 (rn 4) (rt 4) (imm4h 4) 1 0 1 1 (imm4l 4))
+    (:ldrht-encoding-a2 (cond 4) 0 0 0 _ 0 u 0 _ 1 _ 1 (rn 4) (rt 4) (0) (0) (0) (0) 1 0 1 1 (rm 4))
 
-    (:ldrsb-immediate  (cond 4) 0 0 0 p u 1 w 1 (rn 4) (rt 4) (imm4h 4) 1 1 0 1 (imm4l 4))
-    (:ldrsb-literal    (cond 4) 0 0 0 p u 1 w 1 1 1 1 1 (rt 4) (imm4h 4) 1 1 0 1 (imm4l 4))
-    (:ldrsb-register   (cond 4) 0 0 0 p u 0 w 1 (rn 4) (rt 4) (0) (0) (0) (0) 1 1 0 1 (rm 4))
+    (:ldrsb-immediate (cond 4) 0 0 0 p u 1 w 1 (rn 4) (rt 4) (imm4h 4) 1 1 0 1 (imm4l 4))
+    (:ldrsb-literal   (cond 4) 0 0 0 p u 1 w 1 1 1 1 1 (rt 4) (imm4h 4) 1 1 0 1 (imm4l 4))
+    (:ldrsb-register  (cond 4) 0 0 0 p u 0 w 1 (rn 4) (rt 4) (0) (0) (0) (0) 1 1 0 1 (rm 4))
 
-    (:ldrsbt-encoding-a1  (cond 4) 0 0 0   0 u 1 1 1 (rn 4) (rt 4) (imm4h 4) 1 1 0 1 (imm4l 4))
-    (:ldrsbt-encoding-a2  (cond 4) 0 0 0 _ 0 u 0 1 1 (rn 4) (rt 4) (0) (0) (0) (0) 1 1 0 1 (rm 4))
+    (:ldrsbt-encoding-a1 (cond 4) 0 0 0   0 u 1 1 1 (rn 4) (rt 4) (imm4h 4) 1 1 0 1 (imm4l 4))
+    (:ldrsbt-encoding-a2 (cond 4) 0 0 0 _ 0 u 0 1 1 (rn 4) (rt 4) (0) (0) (0) (0) 1 1 0 1 (rm 4))
 
-    (:ldrsh-immediate  (cond 4) 0 0 0 p u 1 w 1 (rn 4) (rt 4) (imm4h 4) 1 1 1 1 (imm4l 4))
-    (:ldrsh-literal    (cond 4) 0 0 0 p u 1 w 1 1 1 1 1 (rt 4) (imm4h 4) 1 1 1 1 (imm4l 4))
-    (:ldrsh-register   (cond 4) 0 0 0 p u 0 w 1 (rn 4) (rt 4) (0) (0) (0) (0) 1 1 1 1 (rm 4))
+    (:ldrsh-immediate (cond 4) 0 0 0 p u 1 w 1 (rn 4) (rt 4) (imm4h 4) 1 1 1 1 (imm4l 4))
+    (:ldrsh-literal   (cond 4) 0 0 0 p u 1 w 1 1 1 1 1 (rt 4) (imm4h 4) 1 1 1 1 (imm4l 4))
+    (:ldrsh-register  (cond 4) 0 0 0 p u 0 w 1 (rn 4) (rt 4) (0) (0) (0) (0) 1 1 1 1 (rm 4))
 
-    (:ldrsht-encoding-a1  (cond 4) 0 0 0   0 u 1   1   1 (rn 4) (rt 4) (imm4h 4) 1 1 1 1 (imm4l 4))
-    (:ldrsht-encoding-a2  (cond 4) 0 0 0 _ 0 u 0 _ 1 _ 1 (rn 4) (rt 4) (0) (0) (0) (0) 1 1 1 1 (rm 4))
+    (:ldrsht-encoding-a1 (cond 4) 0 0 0   0 u 1   1   1 (rn 4) (rt 4) (imm4h 4) 1 1 1 1 (imm4l 4))
+    (:ldrsht-encoding-a2 (cond 4) 0 0 0 _ 0 u 0 _ 1 _ 1 (rn 4) (rt 4) (0) (0) (0) (0) 1 1 1 1 (rm 4))
 
-    (:ldrt-encoding-a1  (cond 4) 0 1 0 0 u 0 1 1 (rn 4) (rt 4) (imm12 12))
-    (:ldrt-encoding-a2  (cond 4) 0 1 1 0 u 0 1 1 (rn 4) (rt 4) (imm5 5) (type 2) 0 (rm 4))
+    (:ldrt-encoding-a1 (cond 4) 0 1 0 0 u 0 1 1 (rn 4) (rt 4) (imm12 12))
+    (:ldrt-encoding-a2 (cond 4) 0 1 1 0 u 0 1 1 (rn 4) (rt 4) (imm5 5) (type 2) 0 (rm 4))
 
-    (:lsl-immediate  (cond 4) 0 0 0 1 1 0 1 s 0 0 0 0 (rd 4) (imm5 5) 0 0 0 (rm 4))
-    (:lsl-register  (cond 4) 0 0 0 1 1 0 1 s 0 0 0 0 (rd 4) (rm 4) 0 0 0 1 (rn 4))
+    (:lsl-immediate (cond 4) 0 0 0 1 1 0 1 s 0 0 0 0 (rd 4) (imm5 5) 0 0 0 (rm 4))
+    (:lsl-register (cond 4) 0 0 0 1 1 0 1 s 0 0 0 0 (rd 4) (rm 4) 0 0 0 1 (rn 4))
 
-    (:lsr-immediate  (cond 4) 0 0 0 1 1 0 1 s 0 0 0 0 (rd 4) (imm5 5) 0 1 0 (rm 4))
-    (:lsr-register  (cond 4) 0 0 0 1 1 0 1 s 0 0 0 0 (rd 4) (rm 4) 0 0 1 1 (rn 4))
+    (:lsr-immediate (cond 4) 0 0 0 1 1 0 1 s 0 0 0 0 (rd 4) (imm5 5) 0 1 0 (rm 4))
+    (:lsr-register (cond 4) 0 0 0 1 1 0 1 s 0 0 0 0 (rd 4) (rm 4) 0 0 1 1 (rn 4))
 
 ;;;    (:mcr  (cond 4) 1 1 1 0 (opc1 3) 0 (crn 4) (rt 4) (coproc 4) (opc2 3) 1 (crm 4))
 ;;;    (:mcr2 1 1 1 1 _ 1 1 1 0 (opc1 3) 0 (crn 4) (rt 4) (coproc 4) (opc2 3) 1 (crm 4))
@@ -184,14 +187,17 @@
     (:movw-immediate  (cond 4) 0 0 1 1 _ 0 0 0 0 (imm4 4) (rd 4) (imm12 12)) ; encoding a2 is movw
     (:mov-register  (cond 4) 0 0 _ 0 1 1 0 1 s (0) (0) (0) (0) (rd 4) 0 0 0 0 0 0 0 0 (rm 4))
 
-;;;    (:movt  (cond 4) 0 0 1 1 0 1 0 0 (imm4 4) (rd 4) (imm12 12))
+    (:movt (cond 4) 0 0 1 1 _ 0 1 0 0 (imm4 4) (rd 4) (imm12 12))
 
-;;;    (:mrc (cond 4) 1 1 1 0 (opc1 3) 1 (crn 4) (rt 4) (coproc 4) (opc2 3) 1 (crm 4)) ; encoding a1 is mrc
-;;;    (:mrc2 1 1 1 1 _ 1 1 1 0 (opc1 3) 1 (crn 4) (rt 4) (coproc 4) (opc2 3) 1 (crm 4)) ; encoding a2 is mrc2
+;;;    (:mrc (cond 4) 1 1 1 0 (opc1 3) 1 (crn 4) (rt 4) (coproc 4) (opc2 3) 1 (crm 4)) ; encoding a1 is mrc ; coprocessors
+;;;    (:mrc2 1 1 1 1 _ 1 1 1 0 (opc1 3) 1 (crn 4) (rt 4) (coproc 4) (opc2 3) 1 (crm 4)) ; encoding a2 is mrc2 ; coprocessors
 
-    ;; todo: mrrc/mrrc2
-    ;; todo: mrs
-    ;; todo: msr
+    ;; todo: mrrc/mrrc2 ; coprocessors
+
+    (:mrs (cond 4) 0 0 0 1 0 _ 0 _ 0 0 (1) (1) (1) (1) (rd 4) (0) (0) 0 (0) 0 0 0 0 (0) (0) (0) (0))
+
+    (:msr-immediate (cond 4) 0 0 1 1 0 _ 0 _ 1 0 (mask 2) 0 0 (1) (1) (1) (1) (imm12 12))
+    (:msr-register  (cond 4) 0 0 0 1 0 _ 0 _ 1 0 (mask 2) 0 0 (1) (1) (1) (1) (0) (0) 0 (0) 0 0 0 0 (rn 4))
 
     (:mul (cond 4) 0 0 0 0 0 0 0 s (rd 4) (0) (0) (0) (0) (rm 4) 1 0 0 1 (rn 4))
 
@@ -326,7 +332,7 @@
     (:sub-register-shifted-register   (cond 4) 0 0 0 0 0 1 0 s (rn 4) (rd 4) (rs 4) 0 (type 2) 1 (rm 4))
     ;; "sub SP minus immediate" and "sub SP minus register" seem to be just special cases of the above
 
-;;;    (:svc (cond 4) 1 1 1 1 (imm24 24))
+;;;    (:svc (cond 4) 1 1 1 1 (imm24 24)) ; supervisor call
 
     ;; todo: swp, swpb
     ;; todo: sxtab
@@ -496,6 +502,7 @@
 (defconst *allowed-encoding-overlaps*
   '((:add-immediate :adr-encoding-a1)
     (:bfc :bfi)
+    (:bl :blx-immediate)
     (:sub-immediate :adr-encoding-a2)
     (:str-immediate :push-encoding-a2)
     (:str-immediate :strt-encoding-a1)
@@ -528,6 +535,7 @@
     (:mov-register :lsl-immediate) ; for the shift=0 case in LSL
     (:mcr :mcr2)
     (:mrc :mrc2)
+    (:msr-immediate :nop)
     (:ldm/ldmia/ldmfd :pop-encoding-a1)
     (:ldr-immediate :pop-encoding-a2)
     (:strb-immediate :strbt-encoding-a1) ; check me
